# Problem 1.
Consider the following facts, rules, and queries.
```
Facts:
  child('Jill','Zed').
  child('Ned','Bea').
  child('Tim','Jack').
  child('Sue','Jack').
  child('Anne','Jill').
  child('Lou','Jane').
  child('Mary','Tim').
  child('Ron','Dan').
  child('Anna','Kim').
  child('Tim','Jill').
  child('Mary','Jane').
  child('Jill','Bea').

Rules:
  ancestor(X,Y) :- child(Y,X).
  ancestor(X,Y) :- child(Y,Z), ancestor(X,Z).

Queries:
  ancestor('Zed','Mary')?
```
a. Write the rules as clauses (disjunctions of literals).
```
ancestor(X,Y) :- child(Y,X).
ancestor(X,Y) :- child(Y,Z), ancestor(X,Z).
```

b. Write one formal proof of the query using proof-by-contradiction, instantiation, and resolution. Give a justification for each line in your proof. Each step must be a premise or the result of instantiation or resolution.
Query: ancestor('Zed','Mary')?

Apply the rule `ancestor(X,Y) :- child(Y,X) with X = 'Zed', Y = 'Mary'` => `child('Mary','Zed')`

Apply the rule `ancestor(X,Y) :- child(Y,Z), ancestor(X,Z)` => `child('Zed', 'Jill'), ancestor('Jill', 'Mary')`

Apply the rule `ancestor(X,Y) :- child(Y,X) with X = 'Jill', Y = 'Mary'` => `child('Mary', 'Jill')`

Apply the rule `ancestor(X,Y) :- child(Y,Z), ancestor(X,Z)` => `child('Jill', 'Tim'), ancestor('Tim', 'Mary')`

Apply the rule `ancestor(X,Y) :- child(Y,X) with X = 'Tim', Y = 'Mary'` => `child('Mary', 'Tim')`

Apply the rule `ancestor(X,Y) :- child(Y,Z), ancestor(X,Z)` => `child('Tim', 'Jill'), ancestor('Jill', 'Mary')`

Apply the rule `ancestor(X,Y) :- child(Y,X) with X = 'Jill', Y = 'Mary'` => `child('Mary', 'Jill')`

Steps 4 and 8 are repeated => This indicates a cycle in the proof, implying that 'Zed' is not an ancestor of 'Mary' and since a contradiction is reached, we can conclude that 'Zed' is not an ancestor of 'Mary'.
